Bdd/Sat.lean
@@ -16,15 +16,11 @@ lemma BDD_of_literal_nvars : (BDD_of_literal (n := n) C).nvars ≤ n := by
 
 @[simp]
 lemma BDD_of_clause_nvars : (BDD_of_clause (n := n) C).nvars ≤ n := by
-  induction C with
-  | nil => simp [BDD_of_clause]
-  | cons head tail ih => simp_all [BDD_of_clause]
+  induction C <;> simp_all [BDD_of_clause]
 
 @[simp]
 lemma BDD_of_CNF_nvars : (BDD_of_CNF (n := n) C).nvars ≤ n := by
-  induction C with
-  | nil => simp [BDD_of_CNF]
-  | cons head tail ih => simp_all [BDD_of_CNF]
+  induction C <;> simp_all [BDD_of_CNF]
 
 lemma BDD_of_CNF_correct {n} {f : Fin n → Bool} (C : Std.Sat.CNF (Fin n)) :
     Std.Sat.CNF.eval f C = (BDD_of_CNF C).denotation (n := n) (by simp) (Vector.ofFn f) := by
@@ -47,49 +43,49 @@ lemma BDD_of_CNF_correct {n} {f : Fin n → Bool} (C : Std.Sat.CNF (Fin n)) :
 
 instance instDecidableUnsat (C : Std.Sat.CNF (Fin n)) : Decidable (Std.Sat.CNF.Unsat C) :=
   decidable_of_iff ((BDD_of_CNF C).SemanticEquiv (BDD.const false)) ⟨l_to_r, r_to_l⟩ where
-  l_to_r h := by
-    simp only [BDD.SemanticEquiv] at h
-    contrapose h
-    rw [funext_iff]
-    simp only [Std.Sat.CNF.Unsat, not_forall, Bool.not_eq_false] at h
-    rcases h with ⟨f, hf⟩
-    rw [BDD_of_CNF_correct] at hf
-    simp only [Fin.eta, BDD.const_nvars, BDD.const_denotation, Function.const_apply, not_forall, Bool.not_eq_false]
-    use Vector.cast (by simp) (Vector.ofFn fun i : Fin (BDD_of_CNF C).nvars ↦ f ⟨i.1, lt_of_lt_of_le i.2 BDD_of_CNF_nvars⟩)
-    simp only [le_refl, BDD.denotation_cast]
-    rw [BDD.denotation_take'] at hf
-    rw [← hf]
-    congr
-    ext i hi
-    have := Vector.getElem_extract (as := (Vector.ofFn f)) (show i < (min (BDD_of_CNF C).nvars n) - 0 by simpa)
-    simp_all
-  r_to_l h := by
-    simp only [Std.Sat.CNF.Unsat] at h
-    simp only [BDD.SemanticEquiv]
-    ext I
-    simp only [BDD.const_nvars, BDD.const_denotation, Function.const_apply]
-    have := h (fun i ↦ if hi : i < (max (BDD_of_CNF C).nvars (BDD.const false).nvars) then I[i] else false)
-    simp only [BDD.const_nvars, zero_le, sup_of_le_left, Fin.getElem_fin] at this
-    rw [BDD_of_CNF_correct] at this
-    rw [BDD.denotation_take (m := max (BDD_of_CNF C).nvars (BDD.const false).nvars)] at this
-    rw [← this]
-    simp only [BDD.const_nvars]
-    conv => lhs; rw [BDD.denotation_take' (hn := by simp)]
-    conv => rhs; rw [BDD.denotation_take' (hn := by simp)]
-    congr 1
-    swap; simp
-    swap; simp
-    simp only [Vector.take_eq_extract, Vector.extract_extract, Nat.add_zero, Nat.sub_zero,
-      Vector.cast_cast, Vector.cast_eq_cast]
-    ext i hi
-    simp only [Nat.sub_zero, Vector.getElem_cast]
-    have := Vector.getElem_extract (as := I) (show i < (min (BDD_of_CNF C).nvars (max (BDD_of_CNF C).nvars (BDD.const false).nvars)) - 0 by simp; omega)
-    simp_all only [BDD.const_nvars, Vector.take_eq_extract, Nat.sub_zero, zero_add]
-    have := Vector.getElem_extract (as := (Vector.ofFn fun i : Fin n ↦ if h : i.1 < (BDD_of_CNF C).nvars then I[i.1] else false)) (show i < min ((min (0 + (BDD_of_CNF C).nvars) (max (BDD_of_CNF C).nvars 0))) n - 0 by simp_all; omega)
-    simp_all only [Nat.sub_zero, BDD.const_nvars, zero_add, Vector.getElem_ofFn]
-    split
-    next => rfl
-    next c => absurd c; omega
+    l_to_r h := by
+      simp only [BDD.SemanticEquiv] at h
+      contrapose h
+      rw [funext_iff]
+      simp only [Std.Sat.CNF.Unsat, not_forall, Bool.not_eq_false] at h
+      rcases h with ⟨f, hf⟩
+      rw [BDD_of_CNF_correct] at hf
+      simp only [Fin.eta, BDD.const_nvars, BDD.const_denotation, Function.const_apply, not_forall, Bool.not_eq_false]
+      use Vector.cast (by simp) (Vector.ofFn fun i : Fin (BDD_of_CNF C).nvars ↦ f ⟨i.1, lt_of_lt_of_le i.2 BDD_of_CNF_nvars⟩)
+      simp only [le_refl, BDD.denotation_cast]
+      rw [BDD.denotation_take'] at hf
+      rw [← hf]
+      congr
+      ext i hi
+      have := Vector.getElem_extract (as := (Vector.ofFn f)) (show i < (min (BDD_of_CNF C).nvars n) - 0 by simpa)
+      simp_all
+    r_to_l h := by
+      simp only [Std.Sat.CNF.Unsat] at h
+      simp only [BDD.SemanticEquiv]
+      ext I
+      simp only [BDD.const_nvars, BDD.const_denotation, Function.const_apply]
+      have := h (fun i ↦ if hi : i < (max (BDD_of_CNF C).nvars (BDD.const false).nvars) then I[i] else false)
+      simp only [BDD.const_nvars, zero_le, sup_of_le_left, Fin.getElem_fin] at this
+      rw [BDD_of_CNF_correct] at this
+      rw [BDD.denotation_take (m := max (BDD_of_CNF C).nvars (BDD.const false).nvars)] at this
+      rw [← this]
+      simp only [BDD.const_nvars]
+      conv => lhs; rw [BDD.denotation_take' (hn := by simp)]
+      conv => rhs; rw [BDD.denotation_take' (hn := by simp)]
+      congr 1
+      swap; simp
+      swap; simp
+      simp only [Vector.take_eq_extract, Vector.extract_extract, Nat.add_zero, Nat.sub_zero,
+        Vector.cast_cast, Vector.cast_eq_cast]
+      ext i hi
+      simp only [Nat.sub_zero, Vector.getElem_cast]
+      have := Vector.getElem_extract (as := I) (show i < (min (BDD_of_CNF C).nvars (max (BDD_of_CNF C).nvars (BDD.const false).nvars)) - 0 by simp; omega)
+      simp_all only [BDD.const_nvars, Vector.take_eq_extract, Nat.sub_zero, zero_add]
+      have := Vector.getElem_extract (as := (Vector.ofFn fun i : Fin n ↦ if h : i.1 < (BDD_of_CNF C).nvars then I[i.1] else false)) (show i < min ((min (0 + (BDD_of_CNF C).nvars) (max (BDD_of_CNF C).nvars 0))) n - 0 by simp_all; omega)
+      simp_all only [Nat.sub_zero, BDD.const_nvars, zero_add, Vector.getElem_ofFn]
+      split
+      next => rfl
+      next c => absurd c; omega
 
 -- #eval Std.Sat.CNF.eval (fun _ : Nat ↦ true) []
 -- #eval Std.Sat.CNF.eval (fun _ : Nat ↦ true) []
